theories/rust_typing/automation.v
@@ -775,6 +775,9 @@ Ltac liSidecond_hook P ::=
 lazymatch P with
   | shelve_hint _ => split; [ unfold shelve_hint; shelve_sidecond |]
   | trait_incl_marker _ => split; [shelve_sidecond |]
+  | fast_eq_hint _ =>
+      split; [
+        unfold spec_instantiate_typaram_fst, spec_instantiate_lft_fst, spec_instantiated; simpl; reflexivity | ]
 end.
 
 (** ** Hints for automation *)
